WIP

src/asynchronous_automata.lean
@@ -67,11 +67,52 @@ def template.read_aux : (inside_outside × vonNeumann) ≃ fin 8 :=
 
 structure template (α : Type) := (to_array : array (8) α)
 
-def template.read {α} (arr : template α) (io : inside_outside) (dir : vonNeumann) : α :=
+def template.read_fun {α} (arr : template α) (io : inside_outside) (dir : vonNeumann) : α :=
   arr.to_array.read (template.read_aux (io, dir))
 
-def template.from_fun {α} (f : inside_outside → vonNeumann → α) : template α :=
+def template.read_inv {α} (f : inside_outside → vonNeumann → α) : template α :=
   ⟨⟨λ ix, function.uncurry f (template.read_aux.inv_fun ix)⟩⟩
+
+lemma equiv.coe_coe_symm {α β} (π : α ≃ β) (b : β) : π (π.symm b) = b :=
+by {
+  cases π,
+  simp,
+  rw π_right_inv,
+}
+
+lemma equiv.coe_symm_coe {α β} (π : α ≃ β) (a : α) : π.symm (π a) = a :=
+by {
+  cases π,
+  simp,
+  rw π_left_inv,
+}
+
+def template.read {α} : template α ≃ (inside_outside → vonNeumann → α) :=
+{ 
+  to_fun := template.read_fun,
+  inv_fun := template.read_inv,
+  left_inv := λ x,
+  by {
+    obtain ⟨⟨f⟩⟩ := x,
+    unfold template.read_fun template.read_inv,
+    congr,
+    funext,
+    unfold function.uncurry template.read_fun,
+    simp,
+    unfold array.read d_array.read,
+  },
+  right_inv := λ f,
+  by {
+    funext,
+    unfold template.read_fun template.read_inv,
+    simp only [equiv.inv_fun_as_coe],
+    unfold array.read d_array.read,
+    simp only,
+    have : ((template.read_aux.symm) (template.read_aux (io, dir))) = (io, dir) := equiv.coe_coe_symm _ _,
+    rw this,
+    rw function.uncurry,
+  }
+}
 
 def ACA_rule (α) := (template α → template α → Prop)
 
@@ -139,7 +180,7 @@ def read_template.aux {n m} {α : Type}
 def read_template {n m} {α : Type} 
   (mat : ACA_board (n+1) (m+1) α)
   (ix : fin (n+1) × fin (m+1)) :
-  template α := template.from_fun (read_template.aux mat ix)
+  template α := template.read.symm (read_template.aux mat ix)
 
 instance : functor template := { 
   map := λ α β f t, ⟨f <$> t.to_array⟩,
@@ -238,7 +279,9 @@ notation `#[` arr:(foldr `,` (h t, array.push_back t h) array.nil `]`) := arr.re
 def array.to_vector {n α} (arr : array n α) : vector α n := 
   ⟨arr.to_list, array.to_list_length arr⟩ 
 
-def ACA_rules.from_list : list (array 2 (array 8 (fin 2))) →  rbmap (template bool) (template bool)
+infix `⇨`:40 := rbmap
+
+def ACA_rules.from_list : list (array 2 (array 8 (fin 2))) → template bool ⇨ template bool
   | l :=
     let to_templates : array 2 (array 8 (fin 2)) → (template bool × template bool) :=
       λ arr, 
@@ -268,7 +311,7 @@ def LHZ_list :=
 		#[#[0,0,1,1,0,1,1,1], #[1,1,0,1,1,1,0,0]]  -- Toggle Memory
   ]
 
-def LHZ_base : rbmap (template bool) (template bool) :=
+def LHZ_base : template bool ⇨ template bool :=
   ACA_rules.from_list LHZ_list
 
 def template.print {α} (to_char : α → char) (t : template α) : string := 
@@ -303,5 +346,199 @@ def write_template {n m : ℕ} {α : Type}
     do
     i_o <- [inside, outside],
     dir <- [N, E, S, W],
-    pure (λ m : ACA_board (n+1) (m+1) α, write_template.aux m ix i_o dir (t.read i_o dir)) in
+    pure (λ m : ACA_board (n+1) (m+1) α, write_template.aux m ix i_o dir (template.read t i_o dir)) in
   action_list.foldl (λ m f, f m) M
+
+open equiv
+
+instance : decidable_eq vonNeumann := equiv.decidable_eq vonNeumann_fin4
+
+def vonNeuman_to.linear_order.aux : (vonNeumann → vonNeumann) ↪ list (fin 4) :=
+  ⟨λ f, (vonNeumann_fin4 ∘ f : vonNeumann → (fin 4)) <$> [N, E, S, W],
+  by {
+    intros f g h,
+    simp at h,
+    rcases h with ⟨h_N, h_E, h_S, h_W⟩,
+    funext x, cases x; assumption
+  }⟩
+
+instance : linear_order (vonNeumann → vonNeumann) :=
+  linear_order.preimage vonNeuman_to.linear_order.aux
+
+def vonNeuman_perm.linear_order.aux : ¡vonNeumann ↪ (vonNeumann → vonNeumann) :=
+  { 
+    to_fun := λ π vn, π vn,
+    inj' := λ π σ h, by {simp at h, apply h}
+  }
+
+instance : linear_order ¡vonNeumann := 
+  linear_order.preimage vonNeuman_perm.linear_order.aux
+
+instance : fintype ¡vonNeumann := fintype_perm
+
+namespace symmetries
+
+abbreviation id' : ¡vonNeumann := equiv.refl _
+
+abbreviation  with_op (l : list ¡vonNeumann) (op : ¡vonNeumann) := l ++ op.trans <$> l 
+
+abbreviation symmetries.to_finset_none : list (¡vonNeumann) := pure id'
+abbreviation symmetries.to_finset_reflect := with_op (pure id') reflect_nh
+abbreviation symmetries.to_finset_rotate2 := with_op (pure id') (rotate_clockwise.trans rotate_clockwise)
+abbreviation symmetries.to_finset_rotate4 := with_op symmetries.to_finset_rotate2 rotate_clockwise
+abbreviation symmetries.to_finset_rotate8 : list (¡vonNeumann):= {}
+abbreviation symmetries.to_finset_rotate4reflect := with_op symmetries.to_finset_rotate4 reflect_nh
+
+-- Yes this one is just {} also
+abbreviation symmetries.to_finset_rotate8reflect := with_op symmetries.to_finset_rotate8 reflect_nh
+
+def to_finset : symmetries → (finset ¡vonNeumann)
+| symmetries.none := symmetries.to_finset_none.to_finset
+| symmetries.rotate2 := symmetries.to_finset_rotate2.to_finset
+| symmetries.rotate4 := symmetries.to_finset_rotate4.to_finset
+| symmetries.rotate8 := symmetries.to_finset_rotate8.to_finset
+| symmetries.rotate4reflect := symmetries.to_finset_rotate4reflect.to_finset
+| symmetries.rotate8reflect := symmetries.to_finset_rotate4reflect.to_finset
+| symmetries.reflect := symmetries.to_finset_reflect.to_finset
+| symmetries.permute := finset.univ
+
+end symmetries
+
+def finset.as_list {α β : Type} (f : list α → β) (p : _) : finset α → β
+  | ⟨ms, ms_no_dup⟩ := quotient.lift f p ms
+
+def on_equiv {α β} (π : α ≃ β) (f : β → β) (a : α) : α := π.symm (f (π a))
+
+lemma on_equiv.id {α β} (π : α ≃ β) (a : α) :
+  on_equiv π id a = a := equiv.coe_coe_symm _ _
+
+@[simp]
+lemma on_equiv.functorial {α β} (π : α ≃ β) (f g : β → β) (a : α) :
+  on_equiv π f (on_equiv π g a) = on_equiv π (f ∘ g) a := 
+by {
+  unfold on_equiv,
+  rw equiv.coe_coe_symm,
+}
+
+def template.precompose {α} (t : template α) (f : vonNeumann → vonNeumann) : template α := 
+  on_equiv template.read (λ t io nv, t io (f nv)) t
+
+def template.precompose_id {α} (t : template α) : t.precompose id = t :=
+by {
+  unfold template.precompose,
+  unfold id,
+  have : (λ (t : inside_outside → vonNeumann → α) (io : inside_outside) (nv : vonNeumann), t io nv) = id,
+  { funext, unfold id},
+  rw this,
+  apply on_equiv.id,
+}
+
+lemma template.precompose_functorial {α} (t : template α) (f g : vonNeumann → vonNeumann) :
+  t.precompose (f ∘ g) = (t.precompose f).precompose g := 
+  by {
+    unfold template.precompose,
+    rw on_equiv.functorial,
+  }
+
+def on_rule {α} (π : ¡vonNeumann) : ¡(template α × template α) :=
+  { 
+    to_fun := λ rule, ⟨rule.1.precompose π, rule.2.precompose π⟩,
+    inv_fun := λ rule, ⟨rule.1.precompose π.symm, rule.2.precompose π.symm⟩,
+    left_inv :=
+    by {
+      intro x,
+      obtain ⟨lhs, rhs⟩ := x,
+      simp only,
+      repeat {rw ← template.precompose_functorial},
+      unfold function.comp,
+      simp_rw equiv.coe_coe_symm π,
+      have : (λ (x : vonNeumann), x) = id := by {funext, simp},
+      simp_rw this,
+      simp_rw template.precompose_id,
+    },
+    right_inv := 
+    by {
+      intro x,
+      obtain ⟨lhs, rhs⟩ := x,
+      simp only,
+      repeat {rw ← template.precompose_functorial},
+      unfold function.comp,
+      simp_rw equiv.coe_symm_coe π,
+      have : (λ (x : vonNeumann), x) = id := by {funext, simp},
+      simp_rw this,
+      simp_rw template.precompose_id,
+    }
+  }
+
+def to_rbmap (α) [linear_order α] (base : list (template α × template α)) (πs : list ¡vonNeumann) := 
+  rbmap_of $ has_seq.seq (πs.map (equiv.to_fun ∘ on_rule)) base
+
+def prod_to_sigma {α β} (p : α × β) : (Σ _ : α, β) := ⟨p.1, p.2⟩
+
+axiom rbmap.ext {α β} [linear_order α] (x y : α ⇨ β) : (∀ a : α, x.find a = y.find a) → x = y
+
+lemma list.cons_cons_eq_append {α} (x y : α) (l : list α) : x :: y :: l = [x, y] ++ l := 
+  by {
+    symmetry,
+    rw list.append_eq_cons_iff,
+    right,
+    use [[y]],
+    split, refl,
+    symmetry,
+    rw list.append_eq_cons_iff,
+    right,
+    use list.nil,
+    split, refl,
+    rw list.nil_append,
+  }
+
+lemma list.sorted_perm_eq {α : Type} [partial_order α] (l₁ l₂ : list α) : 
+  l₁.sorted (≤) → l₂.sorted (≤) → l₁ ~ l₂ → l₁ = l₂ :=
+by {
+  intros s₁ s₂ p,
+  induction p,
+  case nil {refl},
+  case cons {
+    congr,
+    apply p_ih (list.sorted_of_sorted_cons s₁) (list.sorted_of_sorted_cons s₂),
+  },
+  case swap {
+    suffices : p_x = p_y,
+      {congr, exact this.symm, exact this},
+    apply has_le.le.antisymm,
+    cases s₂ with _ _ s_x s₂,
+    apply s_x, left, refl,
+    cases s₁ with _ _ s_y s₁,
+    apply s_y, left, refl,
+    
+  }
+}
+
+lemma list.merge_sort.merge_of_parts {α : Type} [linear_order α] (l₁ l₂ : list α) :
+  let ms := list.merge_sort ((≤) : α → α → Prop) in
+   ms (l₁ ++ l₂) = list.merge (≤) (ms l₁) (ms l₂) :=
+by {
+  simp,
+
+}
+
+def finset.to_sorted_list {α : Type} [linear_order α] (s : finset α) : list α :=
+  s.as_list (list.merge_sort has_le.le) 
+    (by {
+      intros a b p,
+      unfold_projs at p,
+      induction p,
+      case nil {refl},
+      case cons {
+        simp_rw list.merge_sort_eq_insertion_sort at *,
+        simp_rw list.insertion_sort_cons_eq_take_drop,
+        congr; exact p_ih,
+      },
+      {
+        simp_rw list.cons_cons_eq_append,
+      },
+    })
+
+-- def rules.elaborate {α} [linear_order α]
+--   (base : template α ⇨ template α) (sym : symmetries) : template α ⇨ template α :=
+--   sym.to_finset.to_sorted_list
